minuska/theories/naive_interpreter.v
@@ -3,6 +3,7 @@ From Minuska Require Import
     tactics
     spec_syntax
     spec_semantics
+    flatten
 .
 
 (*
@@ -394,129 +395,53 @@ Section with_decidable_signature.
         end
     end.
 
-    Fixpoint try_match_wsc
-        (A B : Set)
-        (try_match_A : A -> B -> option Valuation)
-        (wsc : WithASideCondition A)
-        (g : B)
-        : option Valuation :=
-    match wsc with
-    | wsc_base a => try_match_A a g
-    | wsc_sc wsc' sc =>
-        ρ ← try_match_wsc A B try_match_A wsc' g;
-        if evaluate_sc ρ sc then Some ρ else None
-    end.
+    Print GroundTerm.
+    Print GroundTerm'.
 
-    Definition try_match_OpenTerm_builtin_value:
-        OpenTerm -> builtin_value -> option Valuation
-    := fun φ b =>
-    match φ with
-    | aoo_app _ _ _ => None
-    | aoo_operand _ _ bx => builtin_value_try_match_BuiltinOrVar b bx
-    end.
-
-    Definition try_match_OpenTermWSC_builtin_value:
-        OpenTermWSC -> builtin_value -> option Valuation
-    := try_match_wsc
-        OpenTerm
-        builtin_value
-        try_match_OpenTerm_builtin_value
+    #[global]
+    Instance AppliedOperatorOr'_A_B_fmap (A : Type)
+        : FMap (AppliedOperatorOr' A)
+        := @AppliedOperatorOr'_fmap A
     .
 
-    Print LocalRewrite.
-    Print LhsPattern.
 
-    Definition try_match_OpenTermWSC_AppliedOperator'_symbol_builtin_value:
-        OpenTermWSC →
-        AppliedOperator' symbol builtin_value →
-        option Valuation
-    := try_match_wsc
-        OpenTerm
-        (AppliedOperator' symbol builtin_value)
-        (fun φ t => GroundTerm_try_match_OpenTerm (aoo_app _ _ t) φ)
-    .
-
-    Definition try_match_LhsPattern_GroundTerm:
-        LhsPattern -> GroundTerm -> option Valuation
-    := ApppliedOperatorOr'_try_match_AppliedOperatorOr'
-        symbol
-        OpenTermWSC
-        builtin_value
-        try_match_OpenTermWSC_builtin_value
-        try_match_OpenTermWSC_AppliedOperator'_symbol_builtin_value
-        (fun a b => None)
-    .
-
-    Definition try_match_LhsPattern_builtin_value:
-        LhsPattern -> builtin_value -> option Valuation
-    := fun φ b =>
-    match φ with
-    | aoo_app _ _ _ => None
-    | aoo_operand _ _ o => try_match_OpenTermWSC_builtin_value o b
-    end.
-
-    Definition try_match_LRoOToBOV_builtin_value:
-        LocalRewriteOrOpenTermOrBOV -> builtin_value -> option Valuation
-    := fun φ b =>
-    match φ with
-    | lp_rewrite r => try_match_LhsPattern_builtin_value (lr_from r) b
-    | lp_basicpat φ' => try_match_OpenTerm_builtin_value φ' b
-    | lp_bov bx => builtin_value_try_match_BuiltinOrVar b bx
-    end.
-
-    Definition try_match_lrootobov_aosb:
-        LocalRewriteOrOpenTermOrBOV →
-        AppliedOperator' symbol builtin_value →
-        option Valuation
-    := fun l t =>
-    match l with
-    | lp_rewrite r => try_match_LhsPattern_GroundTerm (lr_from r) (aoo_app _ _ t)
-    | lp_basicpat φ' => GroundTerm_try_match_OpenTerm (aoo_app _ _ t) φ'
-    | lp_bov bx => pure_GroundTerm_try_match_BuiltinOrVar t bx
-    end.
-
-    Definition try_match_uncondrule_lhs:
-        UncondRewritingRule -> GroundTerm -> option Valuation
-    :=
-        ApppliedOperatorOr'_try_match_AppliedOperatorOr'
-            symbol
-            LocalRewriteOrOpenTermOrBOV
-            builtin_value
-            try_match_LRoOToBOV_builtin_value
-            try_match_lrootobov_aosb
-            (fun a b => None)
-    .
-
-    Definition try_match_lhs_rule:
-        RewritingRule -> GroundTerm -> option Valuation
-    :=
-        try_match_wsc
-            UncondRewritingRule
-            GroundTerm
-            try_match_uncondrule_lhs
-    .
-
+    Check AppliedOperatorOr'_fmap.
     Fixpoint evaluate_rhs_pattern
-        (ρ : Valuation)
-        (φ : RhsPattern)
-        : option Element :=
-    match φ with
-    | spat_builtin v => Some (el_builtin v)
-    | spat_sym s => Some (el_appsym (aps_operator s))
-    | spat_app φ1 φ2 =>
-        let oe1 : option Element := (evaluate_rhs_pattern ρ φ1) in
-        let oe2 : option Element := (evaluate_rhs_pattern ρ φ2) in
-        match oe1,oe2 with
-        | Some (el_appsym aps1), Some (el_appsym aps2) =>
-            Some (el_appsym (aps_app_aps aps1 aps2))
-        | Some (el_appsym aps1), Some (el_builtin b) =>
-            Some (el_appsym (aps_app_operand aps1 b))
-        | _,_ => None
+            (ρ : Valuation)
+            (φ : RhsPattern)
+            : GroundTerm :=
+        AppliedOperatorOr'_fmap (Expression_evaluate ρ) φ.
+        match φ with
+        | spat_builtin v => Some (el_builtin v)
+        | spat_sym s => Some (el_appsym (aps_operator s))
+        | spat_app φ1 φ2 =>
+            let oe1 : option Element := (evaluate_rhs_pattern ρ φ1) in
+            let oe2 : option Element := (evaluate_rhs_pattern ρ φ2) in
+            match oe1,oe2 with
+            | Some (el_appsym aps1), Some (el_appsym aps2) =>
+                Some (el_appsym (aps_app_aps aps1 aps2))
+            | Some (el_appsym aps1), Some (el_builtin b) =>
+                Some (el_appsym (aps_app_operand aps1 b))
+            | _,_ => None
+            end
+        | spat_var x => ρ !! x (* Is this necessary when we have FunTerms? *)
+        | spat_ft t => funTerm_evaluate ρ t
         end
-    | spat_var x => ρ !! x (* Is this necessary when we have FunTerms? *)
-    | spat_ft t => funTerm_evaluate ρ t
-    end
     .
+
+    Definition rewrite_with
+        (r : FlattenedRewritingRule)
+        (g : GroundTerm)
+        : option GroundTerm
+    :=
+        ρ ← GroundTerm_try_match_OpenTerm g (fr_from r);
+        if decide (Forall (evaluate_sc ρ) (fr_scs r)) then
+            None
+        else None
+    .
+
+
+ 
 
     Lemma evaluate_rhs_pattern_correct
         (φ : RhsPattern)
